first example with automation

Example_Automatic.thy
@@ -1,23 +1,36 @@
 theory Example_Automatic
-imports "Refine_Imperative_HOL/Sepref_Monadify"
+  imports "Refine_Imperative_HOL/Sepref_Tool" "SepLogicTime_RBTreeBasic.RBTree_Impl"
+    Set_Impl2  
 begin
+ 
 
+lemma set_init_hnr'_short[sepref_fr_rules]:
+  "hn_refine (emp) set_empty emp rbt_set_assn (set_init_SPEC)"
+  sorry
 
-definition set_init_t :: "nat" where "set_init_t = 1"
+lemma set_ins_hnr_abs[sepref_fr_rules]:
+  "hn_refine (hn_ctxt rbt_set_assn S p * hn_val Id x x')
+       (rbt_set_insert x' p)
+       (hn_invalid rbt_set_assn S p * hn_val Id x x') rbt_set_assn (set_ins_SPEC $ x $ S)"
+  sorry
 
-definition set_init_SPEC :: "nat set nrest" where
-  "set_init_SPEC \<equiv> SPECT [{} \<mapsto> set_init_t ]"
+(*
+lemma set_mem_hnr_abs[sepref_fr_rules]:
+  "hn_refine (hn_ctxt rbt_set_assn S p * hn_val Id x x')
+     (rbt_search (x'::nat) p)
+     (hn_ctxt rbt_set_assn S p * hn_val Id x x') Y' ( (set_mem_SPEC $ x $ S))"
+  sorry *)
 
-definition set_ins_t :: "nat\<Rightarrow>nat" where "set_ins_t n = (n+1)"
+definition rbt_mem :: "nat \<Rightarrow> (nat, unit) rbt_node ref option \<Rightarrow> bool Heap" where 
+  "rbt_mem x p = do {
+      f \<leftarrow> rbt_search x p;
+      ureturn (f = Some ()) }"
 
-definition set_ins_SPEC where
-  "set_ins_SPEC x S \<equiv> SPECT [insert x S \<mapsto> set_ins_t (card S)]"
-
-fun set_mem_t :: "nat\<Rightarrow>nat" where "set_mem_t n = (n + 1)"
-
-definition set_mem_SPEC where
-  "set_mem_SPEC x S \<equiv> SPECT [ (x \<in> S) \<mapsto> set_mem_t (card S)]"
-
+lemma set_mem_hnr [sepref_fr_rules]:
+  "hn_refine (hn_ctxt rbt_set_assn S p * hn_val Id x x')
+     (rbt_mem (x'::nat) p)
+     (hn_ctxt rbt_set_assn S p * hn_val Id x x') id_assn ( (set_mem_SPEC $ x $ S))"
+  sorry
 
 
 definition rd_impl1 :: "nat list \<Rightarrow> (nat list) nrest" where
@@ -42,9 +55,158 @@ definition rd_impl1 :: "nat list \<Rightarrow> (nat list) nrest" where
           RETURNT ys
       }"
 
+(* library *) 
 
-schematic_goal "hn_refine \<Gamma> ?c ?\<Gamma>' ?R (rd_impl1 as)"
+lemma zuf: "\<up> True * true =  true"  
+  by (simp add: abel_semigroup.commute assn_ext mult.abel_semigroup_axioms)  
 
+
+fun list_assn :: "('a \<Rightarrow> 'c \<Rightarrow> assn) \<Rightarrow> 'a list \<Rightarrow> 'c list \<Rightarrow> assn" where
+  "list_assn P [] [] = emp"
+| "list_assn P (a#as) (c#cs) = P a c * list_assn P as cs"
+| "list_assn _ _ _ = false"
+
+lemma hn_refine_Zero[sepref_fr_rules]: " hn_refine emp
+           (ureturn (0::nat)) emp
+       (pure Id) (RETURNT $ (0::nat))"
+  unfolding hn_refine_def apply (auto simp: zuf mult.assoc  execute_ureturn pure_def hn_ctxt_def)
+   apply(rule exI[where x=0]) apply (auto simp: zero_enat_def relH_def )      
+    using models_in_range top_assn_rule  
+    by (metis (full_types) mod_false zuf)  
+
+lemma hn_refine_Nil[sepref_fr_rules]: " hn_refine emp
+           (ureturn []) emp
+       (list_assn P) (RETURNT $ [])"
+  unfolding hn_refine_def apply (auto simp: zuf mult.assoc  execute_ureturn pure_def hn_ctxt_def)
+   apply(rule exI[where x=0]) apply (auto simp: zero_enat_def relH_def )      
+    using models_in_range top_assn_rule  
+    by (metis (full_types) mod_false zuf)  
+ 
+
+lemma hn_refine_less[sepref_fr_rules]: " hn_refine
+     (hn_val nat_rel x' x * hn_val nat_rel y' y)
+     (ureturn (y < x))
+     (hn_val nat_rel y' y * hn_val nat_rel x' x)
+     (pure bool_rel) (RETURNT $ ((<) $ y' $ x'))"
+  unfolding hn_refine_def apply (auto simp: zuf mult.assoc  execute_ureturn pure_def hn_ctxt_def)
+   apply(rule exI[where x=0]) apply (auto simp: zero_enat_def relH_def  )      
+    using models_in_range top_assn_rule  
+    by (metis (full_types) SepLogic_Misc.mod_pure_star_dist assn_times_comm)
+
+lemma hn_Pair[sepref_fr_rules]: "hn_refine 
+  (hn_ctxt P1 x1 x1' * hn_ctxt P2 x2 x2')
+  (ureturn (x1',x2'))
+  (hn_invalid P1 x1 x1' * hn_invalid P2 x2 x2')
+  (prod_assn P1 P2)
+  (RETURNT$(Pair$x1$x2))"
+  unfolding hn_refine_def apply (auto simp: zuf mult.assoc  execute_ureturn pure_def hn_ctxt_def)
+   apply(rule exI[where x=0]) apply (auto simp: zero_enat_def relH_def )      
+  apply(rule entailsD)  prefer 2 apply auto
+  sorry
+
+lemma hn_refine_length[sepref_fr_rules]: " hn_refine (hn_val Id xs' xs)
+           (ureturn (length xs))
+       (hn_val Id xs' xs)
+       (pure Id) (RETURNT $ (length $ xs'))"
+  unfolding hn_refine_def apply (auto simp: zuf mult.assoc  execute_ureturn pure_def hn_ctxt_def)
+   apply(rule exI[where x=0]) apply (auto simp: zero_enat_def relH_def )      
+    using models_in_range top_assn_rule  
+    by (metis (full_types) mod_false zuf)  
+
+lemma hn_refine_hd[sepref_fr_rules]: " hn_refine (hn_val Id s' s)
+           (ureturn (hd s))
+       (hn_val Id s' s)
+       (pure Id) (RETURNT $ (hd $ s'))"
+  unfolding hn_refine_def apply (auto simp: zuf mult.assoc  execute_ureturn pure_def hn_ctxt_def)
+   apply(rule exI[where x=0]) apply (auto simp: zero_enat_def relH_def )      
+    using models_in_range top_assn_rule  
+    by (metis (full_types) mod_false zuf)  
+  
+
+lemma hn_refine_tl[sepref_fr_rules]: " hn_refine (hn_val Id s' s)
+           (ureturn (tl s))
+       (hn_val Id s' s)
+       (pure Id) (RETURNT $ (tl $ s'))"
+  unfolding hn_refine_def apply (auto simp: zuf mult.assoc  execute_ureturn pure_def hn_ctxt_def)
+   apply(rule exI[where x=0]) apply (auto simp: zero_enat_def relH_def )      
+    using models_in_range top_assn_rule  
+    by (metis (full_types) mod_false zuf)  
+
+ 
+
+lemma hn_if[sepref_comb_rules]:
+  assumes P: "\<Gamma> \<Longrightarrow>\<^sub>t \<Gamma>1 * hn_val bool_rel a a'"
+  assumes RT: "a \<Longrightarrow> hn_refine (\<Gamma>1 * hn_val bool_rel a a') b' \<Gamma>2b R b"
+  assumes RE: "\<not>a \<Longrightarrow> hn_refine (\<Gamma>1 * hn_val bool_rel a a') c' \<Gamma>2c R c"
+  assumes IMP: "TERM If \<Longrightarrow> \<Gamma>2b \<or>\<^sub>A \<Gamma>2c \<Longrightarrow>\<^sub>t \<Gamma>'"
+  shows "hn_refine \<Gamma> (if a' then b' else c') \<Gamma>' R (If$a$b$c)"
+  using P RT RE IMP[OF TERMI]
+  unfolding APP_def PROTECT2_def 
+  by (rule hnr_If)
+
+
+lemma hnr_cons_rule[sepref_fr_rules]: " hn_refine (hn_ctxt (list_assn P) xs' xs * hn_ctxt P x' x)
+           (ureturn (x#xs))
+       (hn_invalid (list_assn P) xs' xs * hn_invalid P x' x)
+       (list_assn P) (RETURNT $ (Cons $  x' $ xs'))"
+  unfolding hn_refine_def apply (auto simp: zuf mult.assoc  execute_ureturn pure_def hn_ctxt_def)
+   apply(rule exI[where x=0]) apply (auto simp: zero_enat_def relH_def )      
+  using models_in_range top_assn_rule        sorry
+
+lemma prod_assn_ctxt: "prod_assn A1 A2 x y = z \<Longrightarrow> hn_ctxt (prod_assn A1 A2) x y = z"
+  by (simp add: hn_ctxt_def)
+lemma hn_case_prod'[sepref_prep_comb_rule,sepref_comb_rules]:
+  assumes FR: "\<Gamma>\<Longrightarrow>\<^sub>thn_ctxt (prod_assn P1 P2) p' p * \<Gamma>1"
+  assumes Pair: "\<And>a1 a2 a1' a2'. \<lbrakk>p'=(a1',a2')\<rbrakk> 
+    \<Longrightarrow> hn_refine (hn_ctxt P1 a1' a1 * hn_ctxt P2 a2' a2 * \<Gamma>1 * hn_invalid (prod_assn P1 P2) p' p) (f a1 a2) 
+          (hn_ctxt P1' a1' a1 * hn_ctxt P2' a2' a2 * hn_ctxt XX1 p' p * \<Gamma>1') R (f' a1' a2')"
+  shows "hn_refine \<Gamma> (case_prod f p) (hn_ctxt (prod_assn P1' P2') p' p * \<Gamma>1')
+    R (case_prod$(\<lambda>\<^sub>2a b. f' a b)$p')" (is "?G \<Gamma>")
+    apply1 (rule hn_refine_cons_pre[OF FR])
+    apply1 extract_hnr_invalids
+    apply1 (cases p; cases p'; simp add: prod_assn_pair_conv[THEN prod_assn_ctxt])
+    apply (rule hn_refine_cons[OF _ Pair _ entt_refl])
+  subgoal
+    apply (simp add: hn_ctxt_def entailst_def)
+          apply(rule ent_true_drop(2))
+          apply(rule ent_true_drop(2)) apply(rule entails_triv) done
+    applyS simp
+      subgoal
+        apply  (simp add: hn_ctxt_def entailst_def mult.assoc)
+    apply(rule match_first)
+    apply(rule match_first) apply(rotatel)
+    apply(rule match_first)  by simp
+      done
+ 
+
+context 
+  fixes as::"nat list"
+  notes [[sepref_register_adhoc as]]
+  notes [sepref_import_param] = IdI[of as] 
+begin
+
+schematic_goal "hn_refine \<Gamma> (?C::?'a Heap) ?\<Gamma>' ?R (rd_impl1 as)" using [[goals_limit = 3]]
+  unfolding rd_impl1_def
+
+  apply sepref_dbg_preproc
+  apply sepref_dbg_cons_init
+  apply sepref_dbg_id 
+     apply sepref_dbg_monadify
+
+     apply sepref_dbg_opt_init
+
+  apply sepref_dbg_trans_step+ 
+
+  apply sepref_dbg_opt
+  apply sepref_dbg_cons_solve \<comment> \<open>Frame rule, recovering the invalidated list 
+    or pure elements, propagating recovery over the list structure\<close>
+  apply sepref_dbg_cons_solve \<comment> \<open>Trivial frame rule\<close>
+  apply sepref_dbg_constraints
+  done
+
+ 
+
+end
 
 
 end
